cfrontend/Csharpminor.v
@@ -138,7 +138,7 @@ Fixpoint bind_parameters (formals: list ident) (args: list val)
 (** Continuations *)
 
 Inductive cont: Type :=
-  | Kstop: cont                         (**r stop program execution *)
+  | Kstop: list typ -> cont              (**r stop program execution *)
   | Kseq: stmt -> cont -> cont          (**r execute stmt, then cont *)
   | Kblock: cont -> cont                (**r exit a block, then do cont *)
   | Kcall: option ident -> function -> env -> temp_env -> cont -> cont.
@@ -223,7 +223,7 @@ Fixpoint call_cont (k: cont) : cont :=
 
 Definition is_call_cont (k: cont) : Prop :=
   match k with
-  | Kstop => True
+  | Kstop _ => True
   | Kcall _ _ _ _ _ => True
   | _ => False
   end.
@@ -525,7 +525,7 @@ Inductive initial_state (p: program): state -> Prop :=
       Genv.find_symbol ge p.(prog_main) = Some b ->
       Genv.find_funct_ptr ge b = Some f ->
       funsig f = signature_main ->
-      initial_state p (Callstate f nil Kstop m0).
+      initial_state p (Callstate f nil (Kstop nil) m0).
 
 Require Import Conventions.
 
@@ -544,7 +544,7 @@ Require Import Conventions.
 Inductive entry_point (p: program): mem -> state -> val -> list val -> Prop :=
 | initi_core:
     let ge := Genv.globalenv p in
-    forall f fb m0 m1 args stk,
+    forall f fb m0 m1 args targs stk,
       Genv.find_funct_ptr ge fb = Some (Internal f) ->
       (* Assume there are no local variables, this could change*)
       f.(fn_vars) = nil ->
@@ -563,14 +563,14 @@ Inductive entry_point (p: program): mem -> state -> val -> list val -> Prop :=
                            && vals_defined args
                            && zlt (4*(2*(Zlength args))) Int.max_unsigned = true ->*)
       entry_point p m0
-                  (Callstate (Internal f) args Kstop m1) (Vptr fb Ptrofs.zero) args.
+                  (Callstate (Internal f) args (Kstop targs) m1) (Vptr fb Ptrofs.zero) args.
 
 
 (** A final state is a [Returnstate] with an empty continuation. *)
 
 Inductive final_state: state -> int -> Prop :=
-  | final_state_intro: forall r m,
-      final_state (Returnstate (Vint r) Kstop m) r.
+  | final_state_intro: forall r m targs,
+      final_state (Returnstate (Vint r) (Kstop targs) m) r.
 
 (** Wrapping up these definitions in a small-step semantics. *)
 
